Finish proof that ORD-RES-11 is a strategy for regular SCL

Simulation_SCLFOL_Ordered_Resolution/Simulation.thy
@@ -22889,7 +22889,9 @@ inductive ord_res_11_invars where
     "ord_res_10_invars N (U\<^sub>e\<^sub>r, \<F>, \<Gamma>)" and
     "{#} |\<in>| N |\<union>| U\<^sub>e\<^sub>r \<longrightarrow> \<Gamma> = []" and
     "\<forall>C. \<C> = Some C \<longrightarrow> atms_of_cls C |\<subseteq>| atms_of_clss (N |\<union>| U\<^sub>e\<^sub>r)" and
-    "\<forall>C. \<C> = Some C \<longrightarrow> trail_false_cls \<Gamma> C"
+    "\<forall>C. \<C> = Some C \<longrightarrow> trail_false_cls \<Gamma> C" and
+    "atms_of_clss U\<^sub>e\<^sub>r |\<subseteq>| atms_of_clss N" and
+    "\<forall>C |\<in>| \<F>. \<exists>L. is_pos L \<and> linorder_lit.is_maximal_in_mset C L"
 
 lemma ord_res_11_invars_initial_state: "ord_res_11_invars N ({||}, {||}, [], None)"
   by (intro ord_res_11_invars.intros ord_res_10_invars.intros) simp_all
@@ -23135,6 +23137,12 @@ proof (cases N s rule: ord_res_11_invars.cases)
       next
         show "\<And>C. None = Some C \<Longrightarrow> trail_false_cls \<Gamma>' C"
           by  simp
+      next
+        show "atms_of_clss U\<^sub>e\<^sub>r |\<subseteq>| atms_of_clss N"
+          using more_invars by argo
+      next
+        show "\<forall>C|\<in>|\<F>. \<exists>L. is_pos L \<and> ord_res.is_maximal_lit L C"
+          using more_invars by argo
       qed
     next
       case step_hyps: (decide_pos A C \<Gamma>' \<F>')
@@ -23269,6 +23277,17 @@ proof (cases N s rule: ord_res_11_invars.cases)
       next
         show "\<And>C. None = Some C \<Longrightarrow> trail_false_cls \<Gamma>' C"
           by  simp
+      next
+        show "atms_of_clss U\<^sub>e\<^sub>r |\<subseteq>| atms_of_clss N"
+          using more_invars by argo
+      next
+        have "\<exists>L. is_pos L \<and> ord_res.is_maximal_lit L C"
+          using step_hyps
+          by (metis (no_types, lifting) clause_could_propagate_def
+              linorder_cls.is_least_in_ffilter_iff literal.discI(1))
+
+        thus "\<forall>C|\<in>|\<F>'. \<exists>L. is_pos L \<and> ord_res.is_maximal_lit L C"
+          using more_invars \<open>\<F>' = (if _ then \<F> else finsert C \<F>)\<close> by simp
       qed
     next
       case step_hyps: (propagate A C \<Gamma>' \<F>')
@@ -23426,6 +23445,17 @@ proof (cases N s rule: ord_res_11_invars.cases)
       next
         show "\<And>C. None = Some C \<Longrightarrow> trail_false_cls \<Gamma>' C"
           by  simp
+      next
+        show "atms_of_clss U\<^sub>e\<^sub>r |\<subseteq>| atms_of_clss N"
+          using more_invars by argo
+      next
+        have "\<exists>L. is_pos L \<and> ord_res.is_maximal_lit L C"
+          using step_hyps
+          by (metis (no_types, lifting) clause_could_propagate_def
+              linorder_cls.is_least_in_ffilter_iff literal.discI(1))
+
+        thus "\<forall>C|\<in>|\<F>'. \<exists>L. is_pos L \<and> ord_res.is_maximal_lit L C"
+          using more_invars \<open>\<F>' = (if _ then \<F> else finsert C \<F>)\<close> by simp
       qed
     next
       case step_hyps: (conflict D)
@@ -23446,6 +23476,12 @@ proof (cases N s rule: ord_res_11_invars.cases)
           using \<open>linorder_cls.is_least_in_fset _ D\<close>
           unfolding linorder_cls.is_least_in_ffilter_iff
           by  simp
+      next
+        show "atms_of_clss U\<^sub>e\<^sub>r |\<subseteq>| atms_of_clss N"
+          using more_invars by argo
+      next
+        show "\<forall>C|\<in>|\<F>. \<exists>L. is_pos L \<and> ord_res.is_maximal_lit L C"
+          using more_invars by argo
       qed
     next
       case step_hyps: (skip L C n \<Gamma>')
@@ -23528,6 +23564,12 @@ proof (cases N s rule: ord_res_11_invars.cases)
         show "\<And>D. Some C = Some D \<Longrightarrow> trail_false_cls \<Gamma>' D"
           using more_invars \<open>\<C> = Some C\<close> \<open>\<Gamma> = (L, n) # \<Gamma>'\<close> \<open>- L \<notin># C\<close>
           using subtrail_falseI by auto
+      next
+        show "atms_of_clss U\<^sub>e\<^sub>r |\<subseteq>| atms_of_clss N"
+          using more_invars by argo
+      next
+        show "\<And>C. C |\<in>| \<F> \<Longrightarrow> \<exists>L. is_pos L \<and> ord_res.is_maximal_lit L C"
+          using more_invars by metis
       qed
     next
       case step_hyps: (resolution L D \<Gamma>' C)
@@ -23606,6 +23648,12 @@ proof (cases N s rule: ord_res_11_invars.cases)
               unfolding trail_false_cls_def by metis
           qed
         qed
+      next
+        show "atms_of_clss U\<^sub>e\<^sub>r |\<subseteq>| atms_of_clss N"
+          using more_invars by argo
+      next
+        show "\<forall>C |\<in>| \<F>. \<exists>L. is_pos L \<and> ord_res.is_maximal_lit L C"
+          using more_invars by metis
       qed
     next
       case step_hyps: (backtrack L \<Gamma>' C)
@@ -23723,6 +23771,16 @@ proof (cases N s rule: ord_res_11_invars.cases)
       next
         show "\<And>C. None = Some C \<Longrightarrow> trail_false_cls \<Gamma>' C"
           by simp
+      next
+        have "atms_of_cls C |\<subseteq>| atms_of_clss N"
+          by (smt (verit, ccfv_threshold) \<open>atms_of_cls C |\<subseteq>| atms_of_clss (N |\<union>| U\<^sub>e\<^sub>r)\<close>
+              atms_of_clss_def fin_mono fmember_ffUnion_iff fsubsetI funion_iff more_invars(6))
+
+        thus "atms_of_clss (finsert C U\<^sub>e\<^sub>r) |\<subseteq>| atms_of_clss N"
+          using \<open>atms_of_clss U\<^sub>e\<^sub>r |\<subseteq>| atms_of_clss N\<close> by simp
+      next
+        show "\<And>C. C |\<in>| \<F> \<Longrightarrow> \<exists>L. is_pos L \<and> ord_res.is_maximal_lit L C"
+          using more_invars by metis
       qed
     qed
   qed
@@ -24811,25 +24869,9 @@ proof -
   finally show ?thesis .
 qed
 
-(*
-lemma
-  fixes N\<^sub>G :: "'f gclause fset" and \<beta>\<^sub>G :: "'f gterm"
-  fixes N :: "('f, 'v) term clause fset" and \<beta> :: "('f, 'v) term"
-  defines "\<beta> \<equiv> term_of_gterm \<beta>\<^sub>G" and "N \<equiv> cls_of_gcls |`| N\<^sub>G"
-  fixes S S'
-  assumes
-    ball_le_\<beta>\<^sub>G: "\<forall>A\<^sub>G |\<in>| atms_of_clss N\<^sub>G. A\<^sub>G \<preceq>\<^sub>t \<beta>\<^sub>G" and
-    run: "(ord_res_11 N\<^sub>G)\<^sup>*\<^sup>* ({||}, {||}, [], None) S" and
-    step: "ord_res_11 N\<^sub>G S S'"
-  shows "scl_fol.regular_scl N \<beta> (state_of_gstate S) (state_of_gstate S')"
-*)
-
 declare [[try1_schedule = "order presburger linarith algebra argo metis | simp auto blast fast fastforce force meson satx"]]
 
-inductive_cases ord_res_10_invars_tripleE: "ord_res_10_invars N (U, \<F>, \<Gamma>)"
-inductive_cases ord_res_11_invars_quadrupleE: "ord_res_11_invars N (U, \<F>, \<Gamma>, \<C>)"
-
-lemma
+lemma ord_res_11_is_strategy_for_regular_scl:
   fixes
     N\<^sub>G :: "'f gclause fset" and
     N :: "('f, 'v) term clause fset" and
@@ -24844,8 +24886,6 @@ lemma
     "S' \<equiv> state_of_gstate S\<^sub>G'"
   assumes
     ball_le_\<beta>\<^sub>G: "\<forall>A\<^sub>G |\<in>| atms_of_clss N\<^sub>G. A\<^sub>G \<preceq>\<^sub>t \<beta>\<^sub>G" and
-    (* invar: "trail_consistent (fst S\<^sub>G)" and *)
-    (* step: "scl_fol_1 N\<^sub>G S\<^sub>G S\<^sub>G'" *)
     run: "(ord_res_11 N\<^sub>G)\<^sup>*\<^sup>* ({||}, {||}, [], None) S\<^sub>G" and
     step: "ord_res_11 N\<^sub>G S\<^sub>G S\<^sub>G'"
   shows
@@ -24888,6 +24928,22 @@ proof -
 
   have \<C>'_def: "\<C>' = map_option (\<lambda>C\<^sub>G. (cls_of_gcls C\<^sub>G, Var)) \<C>\<^sub>G'"
     using S'_def S\<^sub>G'_def \<open>S' \<equiv> state_of_gstate S\<^sub>G'\<close> by simp
+
+  have "atms_of_clss U\<^sub>G |\<subseteq>| atms_of_clss N\<^sub>G"
+    using \<open>ord_res_11_invars N\<^sub>G S\<^sub>G\<close>[unfolded S\<^sub>G_def]
+    unfolding ord_res_11_invars.simps by simp
+
+  have "atms_of_clss (N\<^sub>G |\<union>| U\<^sub>G) = atms_of_clss N\<^sub>G |\<union>| atms_of_clss U\<^sub>G"
+    by (simp add: atms_of_clss_def fimage_funion)
+
+  also have "\<dots> = atms_of_clss N\<^sub>G"
+    using \<open>atms_of_clss U\<^sub>G |\<subseteq>| atms_of_clss N\<^sub>G\<close> by auto
+
+  finally have "atms_of_clss (N\<^sub>G |\<union>| U\<^sub>G) = atms_of_clss N\<^sub>G" .
+
+  have clauses_in_\<F>_have_pos_max_lit: "\<forall>C|\<in>|\<F>. \<exists>L. is_pos L \<and> ord_res.is_maximal_lit L C"
+    using \<open>ord_res_11_invars N\<^sub>G S\<^sub>G\<close>[unfolded S\<^sub>G_def ord_res_11_invars.simps]
+    by simp
 
   have nex_conflict_if_nbex_trail_false:
     "\<not> fBex (iefac \<F> |`| (N\<^sub>G |\<union>| U\<^sub>G)) (trail_false_cls \<Gamma>\<^sub>G) \<Longrightarrow> \<not> Ex (scl_fol.conflict N \<beta> S)"
@@ -25071,7 +25127,7 @@ proof -
         have "A\<^sub>G |\<in>| atms_of_clss (N\<^sub>G |\<union>| U\<^sub>G)"
           using step_hyps linorder_trm.is_least_in_ffilter_iff by blast
         hence "A\<^sub>G |\<in>| atms_of_clss N\<^sub>G"
-          sorry
+          unfolding \<open>atms_of_clss (N\<^sub>G |\<union>| U\<^sub>G) = atms_of_clss N\<^sub>G\<close> .
         hence "A\<^sub>G \<preceq>\<^sub>t \<beta>\<^sub>G"
           using ball_le_\<beta>\<^sub>G by metis
         moreover have "gterm_of_term A = A\<^sub>G"
@@ -25184,7 +25240,7 @@ proof -
         have "A\<^sub>G |\<in>| atms_of_clss (N\<^sub>G |\<union>| U\<^sub>G)"
           using step_hyps linorder_trm.is_least_in_ffilter_iff by simp
         hence "A\<^sub>G |\<in>| atms_of_clss N\<^sub>G"
-          sorry
+          unfolding \<open>atms_of_clss (N\<^sub>G |\<union>| U\<^sub>G) = atms_of_clss N\<^sub>G\<close> .
         hence "A\<^sub>G \<preceq>\<^sub>t \<beta>\<^sub>G"
           using ball_le_\<beta>\<^sub>G by metis
         moreover have "gterm_of_term A = A\<^sub>G"
@@ -25346,7 +25402,7 @@ proof -
         have "A\<^sub>G |\<in>| atms_of_clss (N\<^sub>G |\<union>| U\<^sub>G)"
           using step_hyps linorder_trm.is_least_in_ffilter_iff by simp
         hence "A\<^sub>G |\<in>| atms_of_clss N\<^sub>G"
-          sorry
+          unfolding \<open>atms_of_clss (N\<^sub>G |\<union>| U\<^sub>G) = atms_of_clss N\<^sub>G\<close> .
         hence "A\<^sub>G \<preceq>\<^sub>t \<beta>\<^sub>G"
           using ball_le_\<beta>\<^sub>G by metis
         moreover have "gterm_of_term A = A\<^sub>G"
@@ -25486,13 +25542,97 @@ proof -
       unfolding U'_def \<open>U\<^sub>G' = U\<^sub>G\<close> U_def ..
 
     have
-      "C\<^sub>G |\<in>| iefac \<F> |`| (N\<^sub>G |\<union>| U\<^sub>G)" and
-      "trail_false_cls \<Gamma>\<^sub>G C\<^sub>G"
+      C\<^sub>G_in: "C\<^sub>G |\<in>| iefac \<F> |`| (N\<^sub>G |\<union>| U\<^sub>G)" and
+      C\<^sub>G_false: "trail_false_cls \<Gamma>\<^sub>G C\<^sub>G" and
+      C\<^sub>G_lt: "\<forall>E\<^sub>G |\<in>| iefac \<F> |`| (N\<^sub>G |\<union>| U\<^sub>G). E\<^sub>G \<noteq> C\<^sub>G \<longrightarrow> trail_false_cls \<Gamma>\<^sub>G E\<^sub>G \<longrightarrow> C\<^sub>G \<prec>\<^sub>c E\<^sub>G"
       using \<open>linorder_cls.is_least_in_fset _ C\<^sub>G\<close>
       unfolding atomize_conj linorder_cls.is_least_in_ffilter_iff by argo
 
-    have "C\<^sub>G |\<in>| N\<^sub>G |\<union>| U\<^sub>G"
-      sorry
+    have "\<nexists>L. is_pos L \<and> ord_res.is_maximal_lit L C\<^sub>G"
+    proof (rule notI , elim exE conjE)
+      fix L :: "'f gliteral"
+      assume "is_pos L" and C\<^sub>G_max_lit: "ord_res.is_maximal_lit L C\<^sub>G"
+
+      have "{#} |\<notin>| iefac \<F> |`| (N\<^sub>G |\<union>| U\<^sub>G)"
+        using C\<^sub>G_lt
+        by (metis (full_types) C\<^sub>G_max_lit bot_fset.rep_eq fBex_fempty linorder_cls.leD
+            linorder_lit.is_maximal_in_mset_iff mempty_lesseq_cls set_mset_empty
+            trail_false_cls_mempty)
+
+      have "trail_false_lit \<Gamma>\<^sub>G L"
+        using C\<^sub>G_max_lit C\<^sub>G_false
+        unfolding linorder_lit.is_maximal_in_mset_iff trail_false_cls_def
+        by metis
+
+      then obtain Ln \<Gamma>\<^sub>G\<^sub>0 where "\<Gamma>\<^sub>G = Ln # \<Gamma>\<^sub>G\<^sub>0"
+        by (metis neq_Nil_conv not_trail_false_Nil(1))
+
+      moreover have
+        AAA: "\<forall>x xs. \<Gamma>\<^sub>G = x # xs \<longrightarrow>
+          ((snd x \<noteq> None) \<longleftrightarrow> fBex (iefac \<F> |`| (N\<^sub>G |\<union>| U\<^sub>G)) (trail_false_cls (x # xs))) \<and>
+          (snd x \<noteq> None \<longrightarrow> is_pos (fst x)) \<and>
+          (\<forall>x \<in> set xs. snd x = None)" and
+        BBB: "(\<forall>\<Gamma>\<^sub>1 Ln \<Gamma>\<^sub>0. \<Gamma>\<^sub>G = \<Gamma>\<^sub>1 @ Ln # \<Gamma>\<^sub>0 \<longrightarrow> snd Ln = None \<longrightarrow>
+          \<not> fBex (iefac \<F> |`| (N\<^sub>G |\<union>| U\<^sub>G)) (trail_false_cls (Ln # \<Gamma>\<^sub>0)))" and
+        \<Gamma>\<^sub>G_sorted: "sorted_wrt (\<lambda>x y. atm_of (fst y) \<prec>\<^sub>t atm_of (fst x)) \<Gamma>\<^sub>G"
+        using \<open>ord_res_11_invars N\<^sub>G S\<^sub>G\<close>[unfolded S\<^sub>G_def ord_res_11_invars.simps
+            ord_res_10_invars.simps]
+        by simp_all
+
+      moreover have "fBex (iefac \<F> |`| (N\<^sub>G |\<union>| U\<^sub>G)) (trail_false_cls \<Gamma>\<^sub>G)"
+        using C\<^sub>G_in C\<^sub>G_false by metis
+
+      ultimately have "snd Ln \<noteq> None" and "is_pos (fst Ln)" and "\<forall>x \<in> set \<Gamma>\<^sub>G\<^sub>0. snd x = None"
+        unfolding atomize_conj by metis
+
+      have "\<not> fBex (iefac \<F> |`| (N\<^sub>G |\<union>| U\<^sub>G)) (trail_false_cls \<Gamma>\<^sub>G\<^sub>0)"
+      proof (cases \<Gamma>\<^sub>G\<^sub>0)
+        case Nil
+        then show ?thesis
+          using \<open>{#} |\<notin>| iefac \<F> |`| (N\<^sub>G |\<union>| U\<^sub>G)\<close>
+          by (metis not_trail_false_Nil(2))
+      next
+        case (Cons x xs)
+        then show ?thesis
+          using \<open>\<Gamma>\<^sub>G = Ln # \<Gamma>\<^sub>G\<^sub>0\<close>
+          using \<open>\<forall>x \<in> set \<Gamma>\<^sub>G\<^sub>0. snd x = None\<close>
+          using BBB[rule_format, of "[Ln]", unfolded append_Cons append_Nil]
+          by simp
+      qed
+
+      hence "\<not> trail_false_cls \<Gamma>\<^sub>G\<^sub>0 C\<^sub>G"
+        using C\<^sub>G_in by metis
+
+      hence "fst Ln = - L"
+        using C\<^sub>G_false C\<^sub>G_max_lit \<Gamma>\<^sub>G_sorted[unfolded \<open>\<Gamma>\<^sub>G = Ln # \<Gamma>\<^sub>G\<^sub>0\<close> sorted_wrt.simps]
+        by (smt (verit, ccfv_SIG) Neg_atm_of_iff \<open>\<Gamma>\<^sub>G = Ln # \<Gamma>\<^sub>G\<^sub>0\<close> atm_of_uminus
+            ord_res.less_lit_simps(4) imageE image_insert insertE
+            linorder_lit.dual_order.strict_trans linorder_lit.is_maximal_in_mset_iff
+            linorder_lit.neq_iff linorder_trm.order.irrefl list.simps(15) literal.collapse(1)
+            ord_res.ground_ordered_resolution_calculus_axioms trail_false_cls_def
+            trail_false_lit_def)
+
+      hence "\<not> is_pos L"
+        using \<open>is_pos (fst Ln)\<close>
+        by (simp add: is_pos_neg_not_is_pos)
+
+      thus False
+        using \<open>is_pos L\<close> by contradiction
+    qed
+
+    hence "C\<^sub>G |\<in>| N\<^sub>G |\<union>| U\<^sub>G"
+    proof -
+      obtain C where "C |\<in>| N\<^sub>G |\<union>| U\<^sub>G" and "C\<^sub>G = iefac \<F> C"
+        using C\<^sub>G_in by blast
+
+      hence "C\<^sub>G = C"
+        using \<open>\<nexists>L. is_pos L \<and> ord_res.is_maximal_lit L C\<^sub>G\<close>
+        by (metis clauses_in_\<F>_have_pos_max_lit ex1_efac_eq_factoring_chain iefac_def
+            ord_res.ground_factorings_preserves_maximal_literal)
+
+      thus ?thesis
+        using \<open>C |\<in>| N\<^sub>G |\<union>| U\<^sub>G\<close> by simp
+    qed
 
     have "scl_fol.conflict N \<beta> S S'"
       unfolding S_def S'_def \<open>\<Gamma>' = \<Gamma>\<close> \<open>U' = U\<close> \<C>_def \<C>'_def \<open>\<C>\<^sub>G = None\<close> \<open>\<C>\<^sub>G' = Some C\<^sub>G\<close> option.map
@@ -25610,10 +25750,6 @@ proof -
         by (metis \<open>ord_res.is_strictly_maximal_lit L\<^sub>G C\<^sub>G\<close> linorder_lit.is_greatest_in_mset_iff
             single_subset_iff)
     qed
-
-    (* have image_mset_diff_strong:
-      "\<And>f A B. inj f \<Longrightarrow> image_mset f (A - B) = image_mset f A - image_mset f B"
-      sorry *)
 
     ultimately have "cls_of_gcls C\<^sub>G - {#lit_of_glit L\<^sub>G#} = cls_of_gcls {#K \<in># C\<^sub>G. K \<noteq> L\<^sub>G#}"
       by (metis \<open>add_mset L\<^sub>G {#y \<in># C\<^sub>G. y \<noteq> L\<^sub>G#} = C\<^sub>G\<close> cls_of_gcls_def image_mset_remove1_mset_if
@@ -25777,1092 +25913,41 @@ proof -
   qed
 qed
 
-(* theorem (in scl_fol_calculus)
-  fixes
-    N :: "('f, 'v) Term.term clause fset" and
-    \<beta> :: "('f, 'v) Term.term" and
-    strategy and strategy_init and proj_state
-  assumes strategy_restricts_regular_scl:
-    "\<And>S S'. strategy N \<beta> S S' \<Longrightarrow> regular_scl N \<beta> (proj_state S) (proj_state S')" and
-    initial_state: "proj_state (strategy_init N \<beta>) = initial_state"
-  shows "wfp_on {S. (strategy N \<beta>)\<^sup>*\<^sup>* (strategy_init N \<beta>) S} (strategy N \<beta>)\<inverse>\<inverse>"
-proof (rule wfp_on_antimono_stronger)
-  show "wfp_on {proj_state S | S. (strategy N \<beta>)\<^sup>*\<^sup>* (strategy_init N \<beta>) S} (regular_scl N \<beta>)\<inverse>\<inverse>"
-  proof (rule wfp_on_subset)
-    show "wfp_on {S. (regular_scl N \<beta>)\<^sup>*\<^sup>* initial_state S} (regular_scl N \<beta>)\<inverse>\<inverse>"
-      using termination_regular_scl by metis
-  next
-    show "{proj_state S | S. (strategy N \<beta>)\<^sup>*\<^sup>* (strategy_init N \<beta>) S} \<subseteq>
-      {S. (regular_scl N \<beta>)\<^sup>*\<^sup>* initial_state S}"
-    proof (intro Collect_mono impI, elim exE conjE)
-      fix s S assume "s = proj_state S" and "(strategy N \<beta>)\<^sup>*\<^sup>* (strategy_init N \<beta>) S"
-      then show "(regular_scl N \<beta>)\<^sup>*\<^sup>* initial_state s"
-        by (metis rtranclp_mono_stronger initial_state strategy_restricts_regular_scl)
-    qed
-  qed
-next
-  show "proj_state ` {S. (strategy N \<beta>)\<^sup>*\<^sup>* (strategy_init N \<beta>) S} \<subseteq>
-    {proj_state S |S. (strategy N \<beta>)\<^sup>*\<^sup>* (strategy_init N \<beta>) S}"
-    by blast
-next
-  show "\<And>S' S. (strategy N \<beta>)\<inverse>\<inverse> S' S \<Longrightarrow> (regular_scl N \<beta>)\<inverse>\<inverse> (proj_state S') (proj_state S)"
-    using strategy_restricts_regular_scl by simp
-qed *)
-
-
-
-
-
-
-
-
-
-
-
-
-
-
-
-
-
-
-
-
-
-section \<open>SCL(FOL)-1 (resolution-driven strategy)\<close>
-
-inductive scl_fol_1 where
-  decide_neg: "\<not> (\<exists>C |\<in>| N |\<union>| U. trail_false_cls \<Gamma> C) \<Longrightarrow>
-    linorder_trm.is_least_in_fset {|A\<^sub>2 |\<in>| atms_of_clss N. \<forall>A\<^sub>1 |\<in>| trail_atms \<Gamma>. A\<^sub>1 \<prec>\<^sub>t A\<^sub>2|} A \<Longrightarrow>
-    \<not> (\<exists>C |\<in>| N |\<union>| U. clause_could_propagate \<Gamma> C (Pos A)) \<Longrightarrow>
-    \<Gamma>' = (Neg A, None) # \<Gamma> \<Longrightarrow>
-    scl_fol_1 N (\<Gamma>, U, None) (\<Gamma>', U, None)" |
-
-  decide_pos: "\<not> (\<exists>C |\<in>| N |\<union>| U. trail_false_cls \<Gamma> C) \<Longrightarrow>
-    linorder_trm.is_least_in_fset {|A\<^sub>2 |\<in>| atms_of_clss N. \<forall>A\<^sub>1 |\<in>| trail_atms \<Gamma>. A\<^sub>1 \<prec>\<^sub>t A\<^sub>2|} A \<Longrightarrow>
-    (\<exists>C |\<in>| N |\<union>| U. clause_could_propagate \<Gamma> C (Pos A)) \<Longrightarrow>
-    \<not> (\<exists>D |\<in>| N |\<union>| U. clause_could_propagate \<Gamma> D (Neg A)) \<Longrightarrow>
-    \<Gamma>' = (Pos A, None) # \<Gamma> \<Longrightarrow>
-    scl_fol_1 N (\<Gamma>, U, None) (\<Gamma>', U, None)" |
-
-  propagate_pos: "\<not> (\<exists>C |\<in>| N |\<union>| U. trail_false_cls \<Gamma> C) \<Longrightarrow>
-    linorder_trm.is_least_in_fset {|A\<^sub>2 |\<in>| atms_of_clss N. \<forall>A\<^sub>1 |\<in>| trail_atms \<Gamma>. A\<^sub>1 \<prec>\<^sub>t A\<^sub>2|} A \<Longrightarrow>
-    linorder_cls.is_least_in_fset {|C |\<in>| N |\<union>| U. clause_could_propagate \<Gamma> C (Pos A)|} C \<Longrightarrow>
-    (\<exists>D |\<in>| N |\<union>| U. clause_could_propagate \<Gamma> D (Neg A)) \<Longrightarrow>
-    \<Gamma>' = (Pos A, Some {#L \<in># C. L \<noteq> Pos A#}) # \<Gamma> \<Longrightarrow>
-    scl_fol_1 N (\<Gamma>, U, None) (\<Gamma>', U, None)" |
-
-  conflict: "linorder_cls.is_least_in_fset {|C |\<in>| N |\<union>| U. trail_false_cls \<Gamma> C|} C \<Longrightarrow>
-    scl_fol_1 N (\<Gamma>, U, None) (\<Gamma>, U, Some C)" |
-
-  skip: "- L \<notin># C \<Longrightarrow>
-    scl_fol_1 N ((L, n) # \<Gamma>, U, Some C) (\<Gamma>, U, Some C)" |
-
-  resolve: "\<Gamma> = (L, Some C) # \<Gamma>' \<Longrightarrow> L = - K \<Longrightarrow>
-    scl_fol_1 N (\<Gamma>, U, Some (add_mset K D)) (\<Gamma>, U, Some (C + D))" |
-
-  backjump: "\<Gamma> = (L, None) # \<Gamma>' \<Longrightarrow> L = - K \<Longrightarrow>
-    scl_fol_1 N (\<Gamma>, U, Some (add_mset K D)) (\<Gamma>', finsert (add_mset K D) U, None)"
-
-lemma "right_unique (scl_fol_1 N)"
-proof (rule right_uniqueI)
-  fix x y z
-  assume step1: "scl_fol_1 N x y" and step2: "scl_fol_1 N x z"
-  show "y = z"
-    using step1
-  proof (cases N x y rule: scl_fol_1.cases)
-    case step1_hyps: (decide_neg U \<Gamma> A \<Gamma>')
-    show ?thesis
-      using step2
-      unfolding \<open>x = (\<Gamma>, U, None)\<close>
-    proof (cases N "(\<Gamma>, U, None :: 'f gterm literal multiset option)" z rule: scl_fol_1.cases)
-      case (decide_neg A2 \<Gamma>2')
-      with step1_hyps show ?thesis
-        by (metis (no_types, lifting) Uniq_D linorder_trm.Uniq_is_least_in_fset)
-    next
-      case (decide_pos A2 \<Gamma>2')
-      with step1_hyps have False
-        by (metis (no_types, lifting) Uniq_D linorder_trm.Uniq_is_least_in_fset)
-      thus ?thesis ..
-    next
-      case (propagate_pos A2 C2 \<Gamma>2')
-      with step1_hyps have False
-        by (metis (no_types, lifting) Uniq_D linorder_trm.Uniq_is_least_in_fset
-            linorder_cls.is_least_in_ffilter_iff)
-      thus ?thesis ..
-    next
-      case (conflict C2)
-      with step1_hyps have False
-        unfolding linorder_cls.is_least_in_ffilter_iff by blast
-      thus ?thesis ..
-    qed
-  next
-    case step1_hyps: (decide_pos U \<Gamma> A \<Gamma>')
-    show ?thesis
-      using step2
-      unfolding \<open>x = (\<Gamma>, U, None)\<close>
-    proof (cases N "(\<Gamma>, U, None :: 'f gterm literal multiset option)" z rule: scl_fol_1.cases)
-      case (decide_neg A2 \<Gamma>2')
-      with step1_hyps have False
-        by (metis (no_types, lifting) Uniq_D linorder_trm.Uniq_is_least_in_fset)
-      thus ?thesis ..
-    next
-      case (decide_pos A2 \<Gamma>2')
-      with step1_hyps show ?thesis
-        by (metis (no_types, lifting) Uniq_D linorder_trm.Uniq_is_least_in_fset)
-    next
-      case (propagate_pos A2 C2 \<Gamma>2')
-      with step1_hyps have False
-        by (metis (no_types, lifting) Uniq_D linorder_trm.Uniq_is_least_in_fset)
-      thus ?thesis ..
-    next
-      case (conflict C2)
-      with step1_hyps have False
-        unfolding linorder_cls.is_least_in_ffilter_iff by blast
-      thus ?thesis ..
-    qed
-  next
-    case step1_hyps: (propagate_pos U \<Gamma> A C \<Gamma>')
-    show ?thesis
-      using step2
-      unfolding \<open>x = (\<Gamma>, U, None)\<close>
-    proof (cases N "(\<Gamma>, U, None :: 'f gterm literal multiset option)" z rule: scl_fol_1.cases)
-      case (decide_neg A2 \<Gamma>2')
-      with step1_hyps have False
-        by (metis (no_types, lifting) Uniq_D linorder_trm.Uniq_is_least_in_fset
-            linorder_cls.is_least_in_ffilter_iff)
-      thus ?thesis ..
-    next
-      case (decide_pos A2 \<Gamma>2')
-      with step1_hyps show ?thesis
-        by (metis (no_types, lifting) Uniq_D linorder_trm.Uniq_is_least_in_fset)
-    next
-      case step2_hyps: (propagate_pos A2 C2 \<Gamma>2')
-      have "A2 = A"
-        using step1_hyps step2_hyps
-        by (metis (no_types, lifting) Uniq_D linorder_trm.Uniq_is_least_in_fset)
-
-      have "C2 = C"
-        using step1_hyps step2_hyps
-        unfolding \<open>A2 = A\<close>
-        by (metis (no_types, lifting) linorder_cls.is_least_in_ffilter_iff
-            linorder_cls.not_less_iff_gr_or_eq)
-
-      have "\<Gamma>2' = \<Gamma>'"
-        using step1_hyps step2_hyps
-        unfolding \<open>A2 = A\<close> \<open>C2 = C\<close> by argo
-
-      thus "y = z"
-        unfolding \<open>y = (\<Gamma>', U, None)\<close> \<open>z = (\<Gamma>2', U, None)\<close>
-        unfolding prod.inject by argo
-    next
-      case (conflict C2)
-      with step1_hyps have False
-        unfolding linorder_cls.is_least_in_ffilter_iff by blast
-      thus ?thesis ..
-    qed
-  next
-    case step1_hyps: (conflict \<Gamma> U C)
-    show ?thesis
-      using step2
-      unfolding \<open>x = (\<Gamma>, U, None)\<close>
-    proof (cases N "(\<Gamma>, U, None :: 'f gterm literal multiset option)" z rule: scl_fol_1.cases)
-      case (decide_neg A2 \<Gamma>2')
-      with step1_hyps have False
-        using linorder_cls.is_least_in_ffilter_iff by metis
-      thus ?thesis ..
-    next
-      case (decide_pos A2 \<Gamma>2')
-      with step1_hyps have False
-        using linorder_cls.is_least_in_ffilter_iff by metis
-      thus ?thesis ..
-    next
-      case (propagate_pos A2 C2 \<Gamma>2')
-      with step1_hyps have False
-        using linorder_cls.is_least_in_ffilter_iff by metis
-      thus ?thesis ..
-    next
-      case (conflict C2)
-      with step1_hyps show ?thesis
-        by (metis Uniq_D linorder_cls.Uniq_is_least_in_fset)
-    qed
-  next
-    case step2_hyps: (skip L C n \<Gamma> U)
-    show ?thesis
-      using step2
-      unfolding \<open>x = ((L, n) # \<Gamma>, U, Some C)\<close>
-    proof (cases N "((L, n) # \<Gamma>, U, Some C)" z rule: scl_fol_1.cases)
-      case skip
-      with step2_hyps show ?thesis
-        by argo
-    next
-      case (resolve L2 C2 \<Gamma>2' K2 D2)
-      with step2_hyps have False
-        by force
-      thus ?thesis ..
-    next
-      case (backjump L2 \<Gamma>2' K2 D2)
-      with step2_hyps have False
-        by force
-      thus ?thesis ..
-    qed
-  next
-    case step2_hyps: (resolve \<Gamma> L C \<Gamma>' K U D)
-    thus ?thesis
-      using step2 by (simp add: scl_fol_1.simps)
-  next
-    case (backjump \<Gamma> L \<Gamma>' K U D)
-    thus ?thesis
-      using step2 by (simp add: scl_fol_1.simps)
-  qed
-qed
-
-lemma
-  fixes
-    N\<^sub>G :: "'f gclause fset" and
-    N :: "('f, 'v) term clause fset" and
-    \<beta>\<^sub>G :: "'f gterm" and
-    \<beta> :: "('f, 'v) term" and
-    S\<^sub>G S\<^sub>G' :: "('f gterm literal \<times> 'f gterm clause option) list \<times> 'f gclause fset \<times> 'f gclause option" and
-    S S' :: "('f, 'v) state"
-  defines
-    "N \<equiv> cls_of_gcls |`| N\<^sub>G" and
-    "\<beta> \<equiv> term_of_gterm \<beta>\<^sub>G" and
-    "S \<equiv> state_of_gstate S\<^sub>G" and
-    "S' \<equiv> state_of_gstate S\<^sub>G'"
-  assumes
-    ball_le_\<beta>\<^sub>G: "\<forall>A\<^sub>G |\<in>| atms_of_clss N\<^sub>G. A\<^sub>G \<preceq>\<^sub>t \<beta>\<^sub>G" and
-    invar: "trail_consistent (fst S\<^sub>G)" and
-    step: "scl_fol_1 N\<^sub>G S\<^sub>G S\<^sub>G'"
-  shows
-    "scl_fol.regular_scl N \<beta> S S'"
-proof -
-  obtain \<Gamma>\<^sub>G U\<^sub>G \<C>\<^sub>G where S\<^sub>G_def: "S\<^sub>G = (\<Gamma>\<^sub>G, U\<^sub>G, \<C>\<^sub>G)"
-    by (metis surj_pair)
-
-  obtain \<Gamma> U \<C> where S_def: "S = (\<Gamma>, U, \<C>)"
-    by (metis surj_pair)
-
-  have \<Gamma>_def: "\<Gamma> = trail_of_gtrail \<Gamma>\<^sub>G"
-    using S_def S\<^sub>G_def \<open>S \<equiv> state_of_gstate S\<^sub>G\<close> by simp
-
-  have U_def: "U = cls_of_gcls |`| U\<^sub>G"
-    using S_def S\<^sub>G_def \<open>S \<equiv> state_of_gstate S\<^sub>G\<close> by simp
-
-  have \<C>_def: "\<C> = map_option (\<lambda>C\<^sub>G. (cls_of_gcls C\<^sub>G, Var)) \<C>\<^sub>G"
-    using S_def S\<^sub>G_def \<open>S \<equiv> state_of_gstate S\<^sub>G\<close> by simp
-
-  obtain \<Gamma>\<^sub>G' U\<^sub>G' \<C>\<^sub>G' where S\<^sub>G'_def: "S\<^sub>G' = (\<Gamma>\<^sub>G', U\<^sub>G', \<C>\<^sub>G')"
-    by (metis surj_pair)
-
-  obtain \<Gamma>' U' \<C>' where S'_def: "S' = (\<Gamma>', U', \<C>')"
-    by (metis surj_pair)
-
-  have \<Gamma>'_def: "\<Gamma>' = map (\<lambda>(L, opt). (lit_of_glit L, map_option (\<lambda>C. (cls_of_gcls C, lit_of_glit L, Var)) opt)) \<Gamma>\<^sub>G'"
-    using S'_def S\<^sub>G'_def \<open>S' \<equiv> state_of_gstate S\<^sub>G'\<close> by simp
-
-  have U'_def: "U' = cls_of_gcls |`| U\<^sub>G'"
-    using S'_def S\<^sub>G'_def \<open>S' \<equiv> state_of_gstate S\<^sub>G'\<close> by simp
-
-  have \<C>'_def: "\<C>' = map_option (\<lambda>C\<^sub>G. (cls_of_gcls C\<^sub>G, Var)) \<C>\<^sub>G'"
-    using S'_def S\<^sub>G'_def \<open>S' \<equiv> state_of_gstate S\<^sub>G'\<close> by simp
-
-  have nex_conflict_if_nbex_trail_false:
-    "\<not> fBex (N\<^sub>G |\<union>| U\<^sub>G) (trail_false_cls \<Gamma>\<^sub>G) \<Longrightarrow> \<not> Ex (scl_fol.conflict N \<beta> S)"
-  proof (elim contrapos_nn exE)
-    fix x :: "('f, 'v) state"
-    assume "scl_fol.conflict N \<beta> S x"
-    thus "fBex (N\<^sub>G |\<union>| U\<^sub>G) (trail_false_cls \<Gamma>\<^sub>G)"
-      unfolding S_def
-    proof (cases N \<beta> "(\<Gamma>, U, \<C>)" x rule: scl_fol.conflict.cases)
-      case (conflictI D \<gamma>)
-
-      obtain D\<^sub>G where "D\<^sub>G |\<in>| N\<^sub>G |\<union>| U\<^sub>G" and D_def: "D = cls_of_gcls D\<^sub>G"
-        using \<open>D |\<in>| N |\<union>| U\<close>
-        unfolding N_def U_def by blast
-
-      moreover have "trail_false_cls \<Gamma>\<^sub>G D\<^sub>G"
-      proof -
-        have "is_ground_cls D"
-          using \<open>D = cls_of_gcls D\<^sub>G\<close> by simp
-        hence "D \<cdot> \<gamma> = D"
-          by simp
-        hence "trail_false_cls \<Gamma> D"
-          using conflictI by argo
-
-        thus ?thesis
-          unfolding \<Gamma>_def D_def
-          unfolding trail_false_cls_nonground_iff_trail_false_cls_ground .
-      qed
-      ultimately show ?thesis by metis
-    qed
-  qed
-
-  have nex_conflict_if_alread_in_conflict: "\<C>\<^sub>G = Some C\<^sub>G \<Longrightarrow> \<not> Ex (scl_fol.conflict N \<beta> S)" for C\<^sub>G
-    unfolding S_def \<C>_def by (simp add: scl_fol.conflict.simps)
-
-  have nex_conflict_if_no_clause_could_propagate_comp:
-    "\<not> Ex (scl_fol.conflict N \<beta> ((lit_of_glit L\<^sub>G, None) # \<Gamma>, U, \<C>))"
-    if
-      nex_false_clause_wrt_\<Gamma>\<^sub>G: "\<not> fBex (N\<^sub>G |\<union>| U\<^sub>G) (trail_false_cls \<Gamma>\<^sub>G)" and
-      ball_lt_atm_L\<^sub>G: "\<forall>x |\<in>| trail_atms \<Gamma>\<^sub>G. x \<prec>\<^sub>t atm_of L\<^sub>G" and
-      nex_clause_that_propagate: "\<not> (\<exists>C|\<in>|N\<^sub>G |\<union>| U\<^sub>G. clause_could_propagate \<Gamma>\<^sub>G C (- L\<^sub>G))"
-    for L\<^sub>G
-  proof (intro notI, elim exE)
-    fix S'' :: "('f, 'v) SCL_FOL.state"
-    assume "scl_fol.conflict N \<beta> ((lit_of_glit L\<^sub>G, None) # \<Gamma>, U, \<C>) S''"
-    thus "False"
-    proof (cases N \<beta> "((lit_of_glit L\<^sub>G, None) # \<Gamma>, U, \<C>)" S'' rule: scl_fol.conflict.cases)
-      case (conflictI D \<gamma>)
-
-      obtain D\<^sub>G where "D\<^sub>G |\<in>| N\<^sub>G |\<union>| U\<^sub>G" and D_def: "D = cls_of_gcls D\<^sub>G"
-        using \<open>D |\<in>| N |\<union>| U\<close> N_def U_def by blast
-
-      have "(lit_of_glit L\<^sub>G :: ('f, 'v) term literal, None) # \<Gamma> = (trail_of_gtrail ((L\<^sub>G, None) # \<Gamma>\<^sub>G) :: ('f, 'v) SCL_FOL.trail)"
-        by (simp add: \<Gamma>_def)
-
-      moreover have "D \<cdot> \<gamma> = cls_of_gcls D\<^sub>G"
-        unfolding D_def by simp
-
-      ultimately have "trail_false_cls (trail_of_gtrail ((L\<^sub>G, None) # \<Gamma>\<^sub>G) :: ('f, 'v) SCL_FOL.trail) (cls_of_gcls D\<^sub>G)"
-        using \<open>trail_false_cls ((lit_of_glit L\<^sub>G, None) # \<Gamma>) (D \<cdot> \<gamma>)\<close> by argo
-
-      hence "trail_false_cls ((L\<^sub>G, None) # \<Gamma>\<^sub>G) D\<^sub>G"
-        using trail_false_cls_nonground_iff_trail_false_cls_ground by blast
-
-      hence "trail_false_cls \<Gamma>\<^sub>G {#K\<^sub>G \<in># D\<^sub>G. K\<^sub>G \<noteq> - L\<^sub>G#}"
-        unfolding trail_false_cls_def trail_false_lit_def
-        by auto
-
-      moreover have "ord_res.is_maximal_lit (- L\<^sub>G) D\<^sub>G"
-        unfolding linorder_lit.is_maximal_in_mset_iff
-      proof (intro conjI ballI impI)
-        show "- L\<^sub>G \<in># D\<^sub>G"
-          using \<open>D\<^sub>G |\<in>| N\<^sub>G |\<union>| U\<^sub>G\<close> \<open>trail_false_cls ((L\<^sub>G, None) # \<Gamma>\<^sub>G) D\<^sub>G\<close> subtrail_falseI
-            nex_false_clause_wrt_\<Gamma>\<^sub>G
-          by blast
-      next
-        fix K\<^sub>G assume "K\<^sub>G \<in># D\<^sub>G" and "K\<^sub>G \<noteq> - L\<^sub>G"
-        hence "trail_false_lit \<Gamma>\<^sub>G K\<^sub>G"
-          using \<open>trail_false_cls \<Gamma>\<^sub>G {#K\<^sub>G \<in># D\<^sub>G. K\<^sub>G \<noteq> - L\<^sub>G#}\<close>
-          unfolding trail_false_cls_def by simp
-        hence "trail_defined_lit \<Gamma>\<^sub>G K\<^sub>G"
-          by (simp add: trail_defined_lit_iff_true_or_false)
-        hence "atm_of K\<^sub>G |\<in>| trail_atms \<Gamma>\<^sub>G"
-          unfolding trail_defined_lit_iff_trail_defined_atm .
-        hence "atm_of K\<^sub>G \<prec>\<^sub>t atm_of L\<^sub>G"
-          using ball_lt_atm_L\<^sub>G by metis
-        hence "K\<^sub>G \<prec>\<^sub>l - L\<^sub>G"
-          by (cases L\<^sub>G; cases K\<^sub>G) simp_all
-        thus "\<not> - L\<^sub>G \<prec>\<^sub>l K\<^sub>G"
-          by order
-      qed
-
-      moreover have "\<not> trail_defined_lit \<Gamma>\<^sub>G (- L\<^sub>G)"
-        by (metis atm_of_uminus linorder_trm.less_irrefl that(2)
-            trail_defined_lit_iff_trail_defined_atm)
-
-      ultimately have "clause_could_propagate \<Gamma>\<^sub>G D\<^sub>G (- L\<^sub>G)"
-        unfolding clause_could_propagate_def by argo
-
-      hence False
-        using \<open>D\<^sub>G |\<in>| N\<^sub>G |\<union>| U\<^sub>G\<close> nex_clause_that_propagate by metis
-
-      thus ?thesis .
-    qed
-  qed
-
-  show ?thesis
-    using \<open>scl_fol_1 N\<^sub>G S\<^sub>G S\<^sub>G'\<close> unfolding S\<^sub>G_def S\<^sub>G'_def
-  proof (cases N\<^sub>G "(\<Gamma>\<^sub>G, U\<^sub>G, \<C>\<^sub>G)" "(\<Gamma>\<^sub>G', U\<^sub>G', \<C>\<^sub>G')" rule: scl_fol_1.cases)
-    case step_hyps: (decide_neg A\<^sub>G)
-
-    define A :: "('f, 'v) term" where
-      "A = term_of_gterm A\<^sub>G"
-
-    let ?f = "(\<lambda>(L, opt). (lit_of_glit L, map_option (\<lambda>C. (cls_of_gcls C, lit_of_glit L, Var)) opt))"
-    have "\<Gamma>' = map ?f \<Gamma>\<^sub>G'"
-      unfolding \<Gamma>'_def ..
-    also have "\<dots> = map ?f ((Neg A\<^sub>G, None) # \<Gamma>\<^sub>G)"
-      unfolding \<open>\<Gamma>\<^sub>G' = (Neg A\<^sub>G, None) # \<Gamma>\<^sub>G\<close> ..
-    also have "\<dots> = ?f (Neg A\<^sub>G, None) # map ?f \<Gamma>\<^sub>G"
-      unfolding list.map ..
-    also have "\<dots> = ?f (Neg A\<^sub>G, None) # \<Gamma>"
-      unfolding \<Gamma>_def ..
-    also have "\<dots> = (lit_of_glit (Neg A\<^sub>G), None) # \<Gamma>"
-      unfolding prod.case option.map ..
-    also have "\<dots> = (Neg (term_of_gterm A\<^sub>G), None) # \<Gamma>"
-      unfolding lit_of_glit_def literal.map ..
-    also have "\<dots> = (Neg A, None) # \<Gamma>"
-      unfolding A_def ..
-    finally have "\<Gamma>' = decide_lit (Neg A) # \<Gamma>"
-      unfolding decide_lit_def .
-
-    have "U' = U"
-      unfolding U'_def \<open>U\<^sub>G' = U\<^sub>G\<close> U_def ..
-
-    have "\<not> Ex (scl_fol.conflict N \<beta> S)"
-      using \<open>\<not> fBex (N\<^sub>G |\<union>| U\<^sub>G) (trail_false_cls \<Gamma>\<^sub>G)\<close> nex_conflict_if_nbex_trail_false by metis
-
-    moreover have "scl_fol.reasonable_scl N \<beta> S S'"
-      unfolding scl_fol.reasonable_scl_def
-    proof (intro conjI impI notI ; (elim exE) ?)
-      have "scl_fol.decide N \<beta> S S'"
-        unfolding S_def S'_def \<open>U' = U\<close> \<C>_def \<C>'_def \<open>\<C>\<^sub>G = None\<close> \<open>\<C>\<^sub>G' = None\<close> option.map
-      proof (rule scl_fol.decideI')
-        show "is_ground_lit (Neg A \<cdot>l Var)"
-          by (simp add: A_def)
-      next
-        have "\<forall>x |\<in>| trail_atms \<Gamma>\<^sub>G. x \<prec>\<^sub>t A\<^sub>G"
-          using step_hyps linorder_trm.is_least_in_ffilter_iff by simp
-        hence "A\<^sub>G |\<notin>| trail_atms \<Gamma>\<^sub>G"
-          by blast
-        hence "A\<^sub>G \<notin> atm_of ` fst ` set \<Gamma>\<^sub>G"
-          unfolding fset_trail_atms .
-        hence "term_of_gterm A\<^sub>G \<notin> term_of_gterm ` atm_of ` fst ` set \<Gamma>\<^sub>G"
-          using inj_image_mem_iff inj_term_of_gterm by metis
-        hence "term_of_gterm A\<^sub>G \<notin> set (map (\<lambda>x. term_of_gterm (atm_of (fst x))) \<Gamma>\<^sub>G)"
-          unfolding image_set list.map_comp comp_def .
-        hence "A \<notin> set (map (\<lambda>x. atm_of (lit_of_glit (fst x))) \<Gamma>\<^sub>G)"
-          unfolding A_def atm_of_lit_of_glit_conv .
-        hence "A \<notin> atm_of ` fst ` set \<Gamma>"
-          unfolding image_set list.map_comp comp_def \<Gamma>_def fst_case_prod_simp .
-        hence "A |\<notin>| trail_atms \<Gamma>"
-          unfolding fset_trail_atms .
-        thus "\<not> trail_defined_lit \<Gamma> (Neg A \<cdot>l Var)"
-          by (simp add: trail_defined_lit_iff_trail_defined_atm)
-      next
-        have "A\<^sub>G |\<in>| atms_of_clss N\<^sub>G"
-          using step_hyps linorder_trm.is_least_in_ffilter_iff by blast
-        hence "A\<^sub>G \<preceq>\<^sub>t \<beta>\<^sub>G"
-          using ball_le_\<beta>\<^sub>G by metis
-        moreover have "gterm_of_term A = A\<^sub>G"
-          by (simp add: A_def)
-        moreover have "gterm_of_term \<beta> = \<beta>\<^sub>G"
-          by (simp add: \<beta>_def)
-        ultimately have "gterm_of_term A \<preceq>\<^sub>t gterm_of_term \<beta>"
-          by argo
-        thus "less_B\<^sup>=\<^sup>= (atm_of (Neg A) \<cdot>a Var) \<beta>"
-          using inj_term_of_gterm[THEN injD]
-          by (auto simp: less_B_def A_def \<beta>_def)
-      next
-        show "\<Gamma>' = trail_decide \<Gamma> (Neg A \<cdot>l Var)"
-          using \<open>\<Gamma>' = decide_lit (Neg A) # \<Gamma>\<close>
-          unfolding subst_lit_id_subst .
-      qed
-
-      thus "scl_fol.scl N \<beta> S S'"
-        unfolding scl_fol.scl_def by argo
-    next
-      fix S'' :: "('f, 'v) SCL_FOL.state"
-      assume "scl_fol.conflict N \<beta> S' S''"
-
-      moreover have "\<nexists>S''. scl_fol.conflict N \<beta> S' S''"
-      proof -
-        have "\<not> Ex (scl_fol.conflict N \<beta> ((lit_of_glit (Neg A\<^sub>G), None) # \<Gamma>, U, \<C>))"
-        proof (rule nex_conflict_if_no_clause_could_propagate_comp)
-          show "\<not> fBex (N\<^sub>G |\<union>| U\<^sub>G) (trail_false_cls \<Gamma>\<^sub>G)"
-            using \<open>\<not> fBex (N\<^sub>G |\<union>| U\<^sub>G) (trail_false_cls \<Gamma>\<^sub>G)\<close> .
-        next
-          show "\<forall>x |\<in>| trail_atms \<Gamma>\<^sub>G. x \<prec>\<^sub>t atm_of (Neg A\<^sub>G)"
-            unfolding literal.sel
-            using step_hyps linorder_trm.is_least_in_fset_iff by simp
-        next
-          show "\<not> (\<exists>C|\<in>|N\<^sub>G |\<union>| U\<^sub>G. clause_could_propagate \<Gamma>\<^sub>G C (- Neg A\<^sub>G))"
-            using \<open>\<not> (\<exists>C|\<in>|N\<^sub>G |\<union>| U\<^sub>G. clause_could_propagate \<Gamma>\<^sub>G C (Pos A\<^sub>G))\<close> by simp
-        qed
-        moreover have "lit_of_glit (Neg A\<^sub>G) = Neg A"
-          unfolding A_def lit_of_glit_def literal.map ..
-        ultimately show ?thesis
-          unfolding S'_def \<open>\<Gamma>' = decide_lit (Neg A) # \<Gamma>\<close> decide_lit_def
-          using \<C>'_def \<C>_def \<open>U' = U\<close> step_hyps(1) step_hyps(3) by argo
-      qed
-
-      ultimately show False
-        by metis
-    qed
-
-    ultimately show ?thesis
-      unfolding scl_fol.regular_scl_def by argo
-  next
-    case step_hyps: (decide_pos A\<^sub>G)
-
-    define A :: "('f, 'v) term" where
-      "A = term_of_gterm A\<^sub>G"
-
-    let ?f = "(\<lambda>(L, opt). (lit_of_glit L, map_option (\<lambda>C. (cls_of_gcls C, lit_of_glit L, Var)) opt))"
-    have "\<Gamma>' = map ?f \<Gamma>\<^sub>G'"
-      unfolding \<Gamma>'_def ..
-    also have "\<dots> = map ?f ((Pos A\<^sub>G, None) # \<Gamma>\<^sub>G)"
-      unfolding \<open>\<Gamma>\<^sub>G' = (Pos A\<^sub>G, None) # \<Gamma>\<^sub>G\<close> ..
-    also have "\<dots> = ?f (Pos A\<^sub>G, None) # map ?f \<Gamma>\<^sub>G"
-      unfolding list.map ..
-    also have "\<dots> = ?f (Pos A\<^sub>G, None) # \<Gamma>"
-      unfolding \<Gamma>_def ..
-    also have "\<dots> = (lit_of_glit (Pos A\<^sub>G), None) # \<Gamma>"
-      unfolding prod.case option.map ..
-    also have "\<dots> = (Pos (term_of_gterm A\<^sub>G), None) # \<Gamma>"
-      unfolding lit_of_glit_def literal.map ..
-    also have "\<dots> = (Pos A, None) # \<Gamma>"
-      unfolding A_def ..
-    finally have "\<Gamma>' = decide_lit (Pos A) # \<Gamma>"
-      unfolding decide_lit_def .
-
-    have "U' = U"
-      unfolding U'_def \<open>U\<^sub>G' = U\<^sub>G\<close> U_def ..
-
-    have "\<not> Ex (scl_fol.conflict N \<beta> S)"
-      using \<open>\<not> fBex (N\<^sub>G |\<union>| U\<^sub>G) (trail_false_cls \<Gamma>\<^sub>G)\<close> nex_conflict_if_nbex_trail_false by metis
-
-    moreover have "scl_fol.reasonable_scl N \<beta> S S'"
-      unfolding scl_fol.reasonable_scl_def
-    proof (intro conjI impI notI ; (elim exE) ?)
-      have "scl_fol.decide N \<beta> S S'"
-        unfolding S_def S'_def \<open>U' = U\<close> \<C>_def \<C>'_def \<open>\<C>\<^sub>G = None\<close> \<open>\<C>\<^sub>G' = None\<close> option.map
-      proof (rule scl_fol.decideI')
-        show "is_ground_lit (Pos A \<cdot>l Var)"
-          by (simp add: A_def)
-      next
-        have "\<forall>x |\<in>| trail_atms \<Gamma>\<^sub>G. x \<prec>\<^sub>t A\<^sub>G"
-          using step_hyps linorder_trm.is_least_in_ffilter_iff by simp
-        hence "A\<^sub>G |\<notin>| trail_atms \<Gamma>\<^sub>G"
-          by blast
-        hence "A\<^sub>G \<notin> atm_of ` fst ` set \<Gamma>\<^sub>G"
-          unfolding fset_trail_atms .
-        hence "term_of_gterm A\<^sub>G \<notin> term_of_gterm ` atm_of ` fst ` set \<Gamma>\<^sub>G"
-          using inj_image_mem_iff inj_term_of_gterm by metis
-        hence "term_of_gterm A\<^sub>G \<notin> set (map (\<lambda>x. term_of_gterm (atm_of (fst x))) \<Gamma>\<^sub>G)"
-          unfolding image_set list.map_comp comp_def .
-        hence "A \<notin> set (map (\<lambda>x. atm_of (lit_of_glit (fst x))) \<Gamma>\<^sub>G)"
-          unfolding A_def atm_of_lit_of_glit_conv .
-        hence "A \<notin> atm_of ` fst ` set \<Gamma>"
-          unfolding image_set list.map_comp comp_def \<Gamma>_def fst_case_prod_simp .
-        hence "A |\<notin>| trail_atms \<Gamma>"
-          unfolding fset_trail_atms .
-        thus "\<not> trail_defined_lit \<Gamma> (Pos A \<cdot>l Var)"
-          by (simp add: trail_defined_lit_iff_trail_defined_atm)
-      next
-        have "A\<^sub>G |\<in>| atms_of_clss N\<^sub>G"
-          using step_hyps linorder_trm.is_least_in_ffilter_iff by simp
-        hence "A\<^sub>G \<preceq>\<^sub>t \<beta>\<^sub>G"
-          using ball_le_\<beta>\<^sub>G by metis
-        moreover have "gterm_of_term A = A\<^sub>G"
-          by (simp add: A_def)
-        moreover have "gterm_of_term \<beta> = \<beta>\<^sub>G"
-          by (simp add: \<beta>_def)
-        ultimately have "gterm_of_term A \<preceq>\<^sub>t gterm_of_term \<beta>"
-          by argo
-        thus "less_B\<^sup>=\<^sup>= (atm_of (Pos A) \<cdot>a Var) \<beta>"
-          using inj_term_of_gterm[THEN injD]
-          by (auto simp: less_B_def A_def \<beta>_def)
-      next
-        show "\<Gamma>' = trail_decide \<Gamma> (Pos A \<cdot>l Var)"
-          using \<open>\<Gamma>' = decide_lit (Pos A) # \<Gamma>\<close>
-          unfolding subst_lit_id_subst .
-      qed
-
-      thus "scl_fol.scl N \<beta> S S'"
-        unfolding scl_fol.scl_def by argo
-    next
-      fix S'' :: "('f, 'v) SCL_FOL.state"
-      assume "scl_fol.conflict N \<beta> S' S''"
-      
-      moreover have "\<nexists>S''. scl_fol.conflict N \<beta> S' S''"
-      proof -
-        have "\<not> Ex (scl_fol.conflict N \<beta> ((lit_of_glit (Pos A\<^sub>G), None) # \<Gamma>, U, \<C>))"
-        proof (rule nex_conflict_if_no_clause_could_propagate_comp)
-          show "\<not> fBex (N\<^sub>G |\<union>| U\<^sub>G) (trail_false_cls \<Gamma>\<^sub>G)"
-            using \<open>\<not> fBex (N\<^sub>G |\<union>| U\<^sub>G) (trail_false_cls \<Gamma>\<^sub>G)\<close> .
-        next
-          show "\<forall>x|\<in>| trail_atms \<Gamma>\<^sub>G. x \<prec>\<^sub>t atm_of (Pos A\<^sub>G)"
-            unfolding literal.sel
-            using step_hyps linorder_trm.is_least_in_ffilter_iff by simp
-        next
-          show "\<not> (\<exists>C|\<in>|N\<^sub>G |\<union>| U\<^sub>G. clause_could_propagate \<Gamma>\<^sub>G C (- Pos A\<^sub>G))"
-            using \<open>\<not> (\<exists>D|\<in>|N\<^sub>G |\<union>| U\<^sub>G. clause_could_propagate \<Gamma>\<^sub>G D (Neg A\<^sub>G))\<close> by simp
-        qed
-        moreover have "lit_of_glit (Pos A\<^sub>G) = Pos A"
-          unfolding A_def lit_of_glit_def literal.map ..
-        ultimately show ?thesis
-          unfolding S'_def \<open>\<Gamma>' = decide_lit (Pos A) # \<Gamma>\<close> decide_lit_def
-          using \<C>'_def \<C>_def \<open>U' = U\<close> step_hyps(1) step_hyps(3) by argo
-      qed
-
-      ultimately show False by metis
-    qed
-
-    ultimately show ?thesis
-      unfolding scl_fol.regular_scl_def by argo
-  next
-    case step_hyps: (propagate_pos A\<^sub>G C\<^sub>G)
-
-    have "C\<^sub>G |\<in>| N\<^sub>G |\<union>| U\<^sub>G" and "clause_could_propagate \<Gamma>\<^sub>G C\<^sub>G (Pos A\<^sub>G)"
-      using step_hyps linorder_cls.is_least_in_fset_iff by simp_all
-
-    define A :: "('f, 'v) term" where
-      "A = term_of_gterm A\<^sub>G"
-
-    define C :: "('f, 'v) term clause" where
-      "C = cls_of_gcls C\<^sub>G"
-
-    have "ord_res.is_maximal_lit (Pos A\<^sub>G) C\<^sub>G" and "trail_false_cls \<Gamma>\<^sub>G {#K \<in># C\<^sub>G. K \<noteq> Pos A\<^sub>G#}"
-      using \<open>clause_could_propagate \<Gamma>\<^sub>G C\<^sub>G (Pos A\<^sub>G)\<close>
-      unfolding clause_could_propagate_def by metis+
-
-    then obtain C\<^sub>G' where "C\<^sub>G = add_mset (Pos A\<^sub>G) C\<^sub>G'"
-      by (metis linorder_lit.is_maximal_in_mset_iff mset_add)
-
-    define C' :: "('f, 'v) term clause" where
-      "C' = cls_of_gcls C\<^sub>G'"
-
-    let ?f = "(\<lambda>(L, opt). (lit_of_glit L, map_option (\<lambda>C. (cls_of_gcls C, lit_of_glit L, Var)) opt))"
-    have "\<Gamma>' = map ?f \<Gamma>\<^sub>G'"
-      unfolding \<Gamma>'_def ..
-    also have "\<dots> = map ?f ((Pos A\<^sub>G, Some {#L \<in># C\<^sub>G. L \<noteq> Pos A\<^sub>G#}) # \<Gamma>\<^sub>G)"
-      unfolding \<open>\<Gamma>\<^sub>G' = (Pos A\<^sub>G, Some {#L \<in># C\<^sub>G. L \<noteq> Pos A\<^sub>G#}) # \<Gamma>\<^sub>G\<close> ..
-    also have "\<dots> = ?f (Pos A\<^sub>G, Some {#L \<in># C\<^sub>G. L \<noteq> Pos A\<^sub>G#}) # map ?f \<Gamma>\<^sub>G"
-      unfolding list.map ..
-    also have "\<dots> = ?f (Pos A\<^sub>G, Some {#L \<in># C\<^sub>G. L \<noteq> Pos A\<^sub>G#}) # \<Gamma>"
-      unfolding \<Gamma>_def ..
-    also have "\<dots> = (lit_of_glit (Pos A\<^sub>G),
-      Some (cls_of_gcls {#L \<in># C\<^sub>G. L \<noteq> Pos A\<^sub>G#}, lit_of_glit (Pos A\<^sub>G), Var)) # \<Gamma>"
-      unfolding prod.case option.map ..
-    also have "\<dots> = (Pos (term_of_gterm A\<^sub>G),
-      Some (cls_of_gcls {#L \<in># C\<^sub>G. L \<noteq> Pos A\<^sub>G#}, Pos (term_of_gterm A\<^sub>G), Var)) # \<Gamma>"
-      unfolding lit_of_glit_def literal.map ..
-    also have "\<dots> = (Pos A, Some (cls_of_gcls {#L \<in># C\<^sub>G. L \<noteq> Pos A\<^sub>G#}, Pos A, Var)) # \<Gamma>"
-      unfolding A_def ..
-    also have "\<dots> = (Pos A, Some (cls_of_gcls {#L \<in># C\<^sub>G. lit_of_glit L \<noteq> Pos A#}, Pos A, Var)) # \<Gamma>"
-      by (metis A_def glit_of_lit_lit_of_glit lit_of_glit_def literal.simps(9))
-    also have "\<dots> = (Pos A, Some ({#L \<in># cls_of_gcls C\<^sub>G. L \<noteq> Pos A#}, Pos A, Var)) # \<Gamma>"
-      unfolding cls_of_gcls_def
-      unfolding image_mset_filter_mset_swap[of "lit_of_glit" "\<lambda>L. L \<noteq> Pos A" C\<^sub>G]
-      unfolding cls_of_gcls_def[symmetric] ..
-    also have "\<dots> = (Pos A \<cdot>l Var, Some ({#L \<in># cls_of_gcls C\<^sub>G. L \<noteq> Pos A#}, Pos A, Var)) # \<Gamma>"
-      by simp
-    also have "\<dots> = (Pos A \<cdot>l Var, Some ({#L \<in># C. L \<noteq> Pos A#}, Pos A, Var)) # \<Gamma>"
-      unfolding C_def ..
-    finally have "\<Gamma>' = propagate_lit (Pos A) {#L \<in># C. L \<noteq> Pos A#} Var # \<Gamma>"
-      unfolding propagate_lit_def .
-
-    have "U' = U"
-      unfolding U'_def \<open>U\<^sub>G' = U\<^sub>G\<close> U_def ..
-
-    have "\<not> Ex (scl_fol.conflict N \<beta> S)"
-      using \<open>\<not> fBex (N\<^sub>G |\<union>| U\<^sub>G) (trail_false_cls \<Gamma>\<^sub>G)\<close> nex_conflict_if_nbex_trail_false by metis
-
-    moreover have "scl_fol.reasonable_scl N \<beta> S S'"
-      unfolding scl_fol.reasonable_scl_def
-    proof (intro conjI impI notI ; (elim exE) ?)
-      have "scl_fol.propagate N \<beta> S S'"
-        unfolding S_def S'_def \<open>U' = U\<close> \<C>_def \<C>'_def \<open>\<C>\<^sub>G = None\<close> \<open>\<C>\<^sub>G' = None\<close> option.map
-      proof (rule scl_fol.propagateI')
-        show "C |\<in>| N |\<union>| U"
-          using \<open>C\<^sub>G |\<in>| N\<^sub>G |\<union>| U\<^sub>G\<close>
-          unfolding C_def N_def U_def by blast
-      next
-        have "C = cls_of_gcls C\<^sub>G"
-          unfolding C_def ..
-        also have "\<dots> = cls_of_gcls (add_mset (Pos A\<^sub>G) C\<^sub>G')"
-          unfolding \<open>C\<^sub>G = add_mset (Pos A\<^sub>G) C\<^sub>G'\<close> ..
-        also have "\<dots> = add_mset (lit_of_glit (Pos A\<^sub>G)) (cls_of_gcls C\<^sub>G')"
-          unfolding cls_of_gcls_def by simp
-        also have "\<dots> = add_mset (lit_of_glit (Pos A\<^sub>G)) C'"
-          unfolding C'_def ..
-        also have "\<dots> = add_mset (Pos (term_of_gterm A\<^sub>G)) C'"
-          unfolding lit_of_glit_def literal.map ..
-        also have "\<dots> = add_mset (Pos A) C'"
-          unfolding A_def ..
-        finally show "C = add_mset (Pos A) C'" .
-
-        show "is_ground_cls (C \<cdot> Var)"
-          by (simp add: C_def)
-
-        have "A\<^sub>G |\<in>| atms_of_clss N\<^sub>G"
-          using step_hyps linorder_trm.is_least_in_ffilter_iff by simp
-        hence "A\<^sub>G \<preceq>\<^sub>t \<beta>\<^sub>G"
-          using ball_le_\<beta>\<^sub>G by metis
-        moreover have "gterm_of_term A = A\<^sub>G"
-          by (simp add: A_def)
-        moreover have "gterm_of_term \<beta> = \<beta>\<^sub>G"
-          by (simp add: \<beta>_def)
-        ultimately have "gterm_of_term A \<preceq>\<^sub>t gterm_of_term \<beta>"
-          by argo
-        hence "less_B\<^sup>=\<^sup>= A \<beta>"
-          by (auto simp: less_B_def A_def \<beta>_def)
-
-        show "\<forall>K\<in>#C \<cdot> Var. less_B\<^sup>=\<^sup>= (atm_of K) \<beta>"
-        proof (intro ballI)
-          fix K :: "('f, 'v) Term.term literal"
-          assume "K \<in># C \<cdot> Var"
-          hence "K \<in># C"
-            by simp
-          then obtain K\<^sub>G where "K\<^sub>G \<in># C\<^sub>G" and K_def: "K = lit_of_glit K\<^sub>G"
-            unfolding C_def cls_of_gcls_def by blast
-
-          have "K\<^sub>G \<preceq>\<^sub>l Pos A\<^sub>G"
-            using \<open>ord_res.is_maximal_lit (Pos A\<^sub>G) C\<^sub>G\<close> \<open>K\<^sub>G \<in># C\<^sub>G\<close>
-            using linorder_lit.is_maximal_in_mset_iff by auto
-
-          hence "atm_of K\<^sub>G \<preceq>\<^sub>t A\<^sub>G"
-            by (metis literal.collapse(1) literal.collapse(2) literal.sel(1)
-                ord_res.less_lit_simps(1) ord_res.less_lit_simps(4) reflclp_iff)
-
-          hence "less_B\<^sup>=\<^sup>= (atm_of K) A"
-            by (auto simp: less_B_def K_def A_def atm_of_lit_of_glit_conv)
-
-          then show "less_B\<^sup>=\<^sup>= (atm_of K) \<beta>"
-            using \<open>less_B\<^sup>=\<^sup>= A \<beta>\<close> by order
-        qed
-
-        show "{#K \<in># C'. K \<noteq> Pos A#} = {#K \<in># C'. K \<cdot>l Var \<noteq> Pos A \<cdot>l Var#}"
-          by simp
-
-        show "{#K \<in># C'. K = Pos A#} = {#K \<in># C'. K \<cdot>l Var = Pos A \<cdot>l Var#}"
-          by simp
-
-        have "trail_false_cls \<Gamma>\<^sub>G ({#K\<^sub>G \<in># C\<^sub>G'. K\<^sub>G \<noteq> Pos A\<^sub>G#})"
-          using \<open>C\<^sub>G = add_mset (Pos A\<^sub>G) C\<^sub>G'\<close> \<open>trail_false_cls \<Gamma>\<^sub>G {#K \<in># C\<^sub>G. K \<noteq> Pos A\<^sub>G#}\<close> by fastforce
-
-        hence "trail_false_cls \<Gamma> (cls_of_gcls {#K\<^sub>G \<in># C\<^sub>G'. K\<^sub>G \<noteq> Pos A\<^sub>G#} :: ('f, 'v) term clause)"
-          unfolding \<Gamma>_def
-          using trail_false_cls_nonground_iff_trail_false_cls_ground by blast
-
-        moreover have "(cls_of_gcls {#K\<^sub>G \<in># C\<^sub>G'. K\<^sub>G \<noteq> Pos A\<^sub>G#} :: ('f, 'v) term clause) = {#K \<in># C'. K \<noteq> Pos A#}"
-        proof -
-          have "{#K \<in># C'. K \<noteq> Pos A#} = cls_of_gcls {#K \<in># C\<^sub>G'. lit_of_glit K \<noteq> Pos A#}"
-            unfolding C'_def cls_of_gcls_def
-            by (simp add: filter_mset_neq)
-          also have "\<dots> = cls_of_gcls {#K\<^sub>G \<in># C\<^sub>G'. K\<^sub>G \<noteq> Pos A\<^sub>G#}"
-            unfolding A_def
-            by (metis glit_of_lit_lit_of_glit lit_of_glit_def literal.simps(9))
-          finally show ?thesis
-            by argo
-        qed
-
-        ultimately show "trail_false_cls \<Gamma> ({#K \<in># C'. K \<noteq> Pos A#} \<cdot> Var)"
-          by simp
-
-        have "\<forall>x |\<in>| trail_atms \<Gamma>\<^sub>G. x \<prec>\<^sub>t A\<^sub>G"
-          using step_hyps linorder_trm.is_least_in_ffilter_iff by simp
-        hence "A\<^sub>G |\<notin>| trail_atms \<Gamma>\<^sub>G"
-          by blast
-        hence "A\<^sub>G \<notin> atm_of ` fst ` set \<Gamma>\<^sub>G"
-          unfolding fset_trail_atms .
-        hence "term_of_gterm A\<^sub>G \<notin> term_of_gterm ` atm_of ` fst ` set \<Gamma>\<^sub>G"
-          using inj_image_mem_iff inj_term_of_gterm by metis
-        hence "term_of_gterm A\<^sub>G \<notin> set (map (\<lambda>x. term_of_gterm (atm_of (fst x))) \<Gamma>\<^sub>G)"
-          unfolding image_set list.map_comp comp_def .
-        hence "A \<notin> set (map (\<lambda>x. atm_of (lit_of_glit (fst x))) \<Gamma>\<^sub>G)"
-          unfolding A_def atm_of_lit_of_glit_conv .
-        hence "A \<notin> atm_of ` fst ` set \<Gamma>"
-          unfolding image_set list.map_comp comp_def \<Gamma>_def fst_case_prod_simp .
-        hence "A |\<notin>| trail_atms \<Gamma>"
-          unfolding fset_trail_atms .
-        thus "\<not> trail_defined_lit \<Gamma> (Pos A \<cdot>l Var)"
-          by (simp add: trail_defined_lit_iff_trail_defined_atm)
-
-        have FOO: "set_mset (add_mset (Pos A) {#K \<in># C'. K = Pos A#}) = {Pos A}"
-          by auto
-        have "is_unifier Var (atm_of ` set_mset (add_mset (Pos A) {#K \<in># C'. K = Pos A#}))"
-          unfolding FOO
-          by (simp add: SCL_FOL.is_unifier_def)
-        hence "is_unifiers Var {atm_of ` set_mset (add_mset (Pos A) {#K \<in># C'. K = Pos A#})}"
-          unfolding SCL_FOL.is_unifiers_def by simp
-        thus "SCL_FOL.is_imgu Var {atm_of ` set_mset (add_mset (Pos A) {#K \<in># C'. K = Pos A#})}"
-          unfolding SCL_FOL.is_imgu_def by simp
-
-        show "\<Gamma>' = trail_propagate \<Gamma> (Pos A \<cdot>l Var) ({#K \<in># C'. K \<noteq> Pos A#} \<cdot> Var) Var"
-          using \<open>\<Gamma>' = propagate_lit (Pos A) {#L \<in># C. L \<noteq> Pos A#} Var # \<Gamma>\<close>
-          using \<open>C = add_mset (Pos A) C'\<close>
-          by simp
-      qed
-
-      thus "scl_fol.scl N \<beta> S S'"
-        unfolding scl_fol.scl_def by argo
-    next
-      fix S'' :: "('f, 'v) SCL_FOL.state"
-      assume "scl_fol.decide N \<beta> S S'"
-      thus False
-        unfolding S_def S'_def
-      proof (cases N \<beta> "(\<Gamma>, U, \<C>)" "(\<Gamma>', U', \<C>')" rule: scl_fol.decide.cases)
-        case (decideI L \<gamma>)
-        show False
-          using \<open>\<Gamma>' = decide_lit (L \<cdot>l \<gamma>) # \<Gamma>\<close>
-          using \<open>\<Gamma>' = propagate_lit (Pos A) {#L \<in># C. L \<noteq> Pos A#} Var # \<Gamma>\<close>
-          unfolding decide_lit_def propagate_lit_def
-          by blast
-      qed
-    qed
-
-    ultimately show ?thesis
-      unfolding scl_fol.regular_scl_def by argo
-  next
-    case step_hyps: (conflict C\<^sub>G)
-
-    have "\<Gamma>' = \<Gamma>"
-      unfolding \<Gamma>'_def \<open>\<Gamma>\<^sub>G' = \<Gamma>\<^sub>G\<close> \<Gamma>_def ..
-
-    have "U' = U"
-      unfolding U'_def \<open>U\<^sub>G' = U\<^sub>G\<close> U_def ..
-
-    have "scl_fol.conflict N \<beta> S S'"
-      unfolding S_def S'_def \<open>\<Gamma>' = \<Gamma>\<close> \<open>U' = U\<close> \<C>_def \<C>'_def \<open>\<C>\<^sub>G = None\<close> \<open>\<C>\<^sub>G' = Some C\<^sub>G\<close> option.map
-    proof (rule scl_fol.conflictI)
-      show "cls_of_gcls C\<^sub>G |\<in>| N |\<union>| U"
-        unfolding N_def U_def
-        by (metis fimage_funion finsert_fimage finsert_iff linorder_cls.is_least_in_fset_ffilterD(1)
-            step_hyps(5))
-    next
-      show "is_ground_cls (cls_of_gcls C\<^sub>G \<cdot> (Var::'v \<Rightarrow> ('f, _) Term.term))"
+lemma "wfp_on {S. (ord_res_11 N)\<^sup>*\<^sup>* ({||}, {||}, [], None) S} (ord_res_11 N)\<inverse>\<inverse>"
+proof (rule scl_fol.termination_projectable_strategy)
+  fix S S'
+  assume run: "(ord_res_11 N)\<^sup>*\<^sup>* ({||}, {||}, [], None) S" and step: "ord_res_11 N S S'"
+
+  term "atms_of_clss N"
+
+  define \<beta> :: "'f gterm" where
+    "\<beta> = (THE A. linorder_trm.is_greatest_in_fset (atms_of_clss N) A)"
+
+  show "scl_fol.regular_scl (cls_of_gcls |`| N) (term_of_gterm \<beta>) (state_of_gstate S) (state_of_gstate S')"
+  proof (rule ord_res_11_is_strategy_for_regular_scl)
+    show "\<forall>A\<^sub>G |\<in>| atms_of_clss N. A\<^sub>G \<preceq>\<^sub>t \<beta>"
+    proof (cases "atms_of_clss N = {||}")
+      case True
+      thus ?thesis
         by simp
     next
-      have "trail_false_cls \<Gamma>\<^sub>G C\<^sub>G"
-        using linorder_cls.is_least_in_fset_iff step_hyps(5) by force
-
-      thus "trail_false_cls \<Gamma> (cls_of_gcls C\<^sub>G \<cdot> Var)"
-        using \<Gamma>'_def \<open>\<Gamma>' = \<Gamma>\<close> step_hyps(2) trail_false_cls_nonground_iff_trail_false_cls_ground
-        by simp
+      case False
+      then show ?thesis
+        unfolding \<beta>_def
+        by (metis (full_types) linorder_trm.Uniq_is_greatest_in_fset
+            linorder_trm.ex_greatest_in_fset linorder_trm.is_greatest_in_fset_iff sup2CI
+            the1_equality')
     qed
-
-    thus ?thesis
-      unfolding scl_fol.regular_scl_def by argo
   next
-    case step_hyps: (skip L\<^sub>G C\<^sub>G n\<^sub>G)
-
-    have "\<Gamma> = (lit_of_glit L\<^sub>G, map_option (\<lambda>C. (cls_of_gcls C, lit_of_glit L\<^sub>G, Var)) n\<^sub>G) # \<Gamma>'"
-      unfolding \<Gamma>_def \<Gamma>'_def \<open>\<Gamma>\<^sub>G = (L\<^sub>G, n\<^sub>G) # \<Gamma>\<^sub>G'\<close> by auto
-
-    have "U' = U"
-      unfolding U'_def \<open>U\<^sub>G' = U\<^sub>G\<close> U_def ..
-
-    have "\<not> Ex (scl_fol.conflict N \<beta> S)"
-      using \<open>\<C>\<^sub>G = Some C\<^sub>G\<close> nex_conflict_if_alread_in_conflict by metis
-
-    moreover have "scl_fol.reasonable_scl N \<beta> S S'"
-      unfolding scl_fol.reasonable_scl_def
-    proof (intro conjI impI notI ; (elim exE) ?)
-      have "scl_fol.skip N \<beta> S S'"
-        unfolding S_def S'_def \<open>U' = U\<close> \<C>_def \<C>'_def \<open>\<C>\<^sub>G = Some C\<^sub>G\<close> \<open>\<C>\<^sub>G' = Some C\<^sub>G\<close> option.map
-        unfolding \<open>\<Gamma> = (lit_of_glit L\<^sub>G, map_option (\<lambda>C. (cls_of_gcls C, lit_of_glit L\<^sub>G, Var)) n\<^sub>G) # \<Gamma>'\<close>
-      proof (rule scl_fol.skipI)
-        have "- lit_of_glit L\<^sub>G = lit_of_glit (- L\<^sub>G)"
-          by (cases L\<^sub>G) (simp_all add: lit_of_glit_def)
-        show "- lit_of_glit L\<^sub>G \<notin># cls_of_gcls C\<^sub>G \<cdot> Var"
-          unfolding subst_cls_id_subst
-          unfolding \<open>- lit_of_glit L\<^sub>G = lit_of_glit (- L\<^sub>G)\<close>
-          unfolding cls_of_gcls_def
-          using \<open>- L\<^sub>G \<notin># C\<^sub>G\<close> inj_image_mset_mem_iff[OF inj_lit_of_glit]
-          by metis
-      qed
-
-      thus "scl_fol.scl N \<beta> S S'"
-        unfolding scl_fol.scl_def by argo
-    next
-      fix S'' :: "('f, 'v) SCL_FOL.state"
-      assume "scl_fol.conflict N \<beta> S' S''"
-
-      moreover have "\<nexists>S''. scl_fol.conflict N \<beta> S' S''"
-        unfolding S'_def \<C>'_def \<open>\<C>\<^sub>G' = Some C\<^sub>G\<close> by (simp add: scl_fol.conflict.simps)
-
-      ultimately show False
-        by metis
-    qed
-
-    ultimately show ?thesis
-      unfolding scl_fol.regular_scl_def by argo
+    show "(ord_res_11 N)\<^sup>*\<^sup>* ({||}, {||}, [], None) S"
+      using run .
   next
-    case step_hyps: (resolve L\<^sub>G C\<^sub>G \<Gamma>\<^sub>G'' K\<^sub>G D\<^sub>G)
-
-    have "\<Gamma>' = \<Gamma>"
-      unfolding \<Gamma>'_def \<open>\<Gamma>\<^sub>G' = \<Gamma>\<^sub>G\<close> \<Gamma>_def ..
-
-    have "U' = U"
-      unfolding U'_def \<open>U\<^sub>G' = U\<^sub>G\<close> U_def ..
-
-    have "\<C> = Some (add_mset (lit_of_glit K\<^sub>G) (cls_of_gcls D\<^sub>G), Var)"
-      unfolding \<C>_def
-      unfolding \<open>\<C>\<^sub>G = Some (add_mset K\<^sub>G D\<^sub>G)\<close> \<open>\<C>\<^sub>G' = Some (C\<^sub>G + D\<^sub>G)\<close> option.map
-      by (simp add: cls_of_gcls_def)
-
-    have "\<C>' = Some (cls_of_gcls C\<^sub>G + cls_of_gcls D\<^sub>G, Var)"
-      unfolding \<C>'_def \<open>\<C>\<^sub>G' = Some (C\<^sub>G + D\<^sub>G)\<close> option.map
-      by (simp add: cls_of_gcls_def)
-    hence "\<C>' = Some ((cls_of_gcls D\<^sub>G \<cdot> Var + cls_of_gcls C\<^sub>G \<cdot> Var) \<cdot> Var, Var)"
-      by simp
-
-    have "\<not> Ex (scl_fol.conflict N \<beta> S)"
-      using \<open>\<C>\<^sub>G = Some (add_mset K\<^sub>G D\<^sub>G)\<close> nex_conflict_if_alread_in_conflict by metis
-
-    moreover have "scl_fol.reasonable_scl N \<beta> S S'"
-      unfolding scl_fol.reasonable_scl_def
-    proof (intro conjI impI notI ; (elim exE) ?)
-      have "scl_fol.resolve N \<beta> S S'"
-        unfolding S_def S'_def \<open>\<Gamma>' = \<Gamma>\<close> \<open>U' = U\<close>
-        unfolding \<open>\<C> = Some (add_mset (lit_of_glit K\<^sub>G) (cls_of_gcls D\<^sub>G), Var)\<close>
-        unfolding \<open>\<C>' = Some ((cls_of_gcls D\<^sub>G \<cdot> Var + cls_of_gcls C\<^sub>G \<cdot> Var) \<cdot> Var, Var)\<close>
-      proof (rule scl_fol.resolveI)
-        show "\<Gamma> = trail_propagate (trail_of_gtrail \<Gamma>\<^sub>G'') (lit_of_glit L\<^sub>G) (cls_of_gcls C\<^sub>G) Var"
-          unfolding \<Gamma>_def \<open>\<Gamma>\<^sub>G = (L\<^sub>G, Some C\<^sub>G) # \<Gamma>\<^sub>G''\<close> list.map prod.case
-          by (simp add: propagate_lit_def)
-      next
-        show "lit_of_glit L\<^sub>G \<cdot>l Var = - (lit_of_glit K\<^sub>G \<cdot>l Var)"
-          unfolding subst_lit_id_subst
-          using \<open>L\<^sub>G = - K\<^sub>G\<close>
-          by (metis atm_of_eq_atm_of atm_of_lit_of_glit_conv glit_of_lit_lit_of_glit uminus_not_id')
-      next
-        show "SCL_FOL.is_renaming Var"
-          by simp
-      next
-        show "SCL_FOL.is_renaming Var"
-          by simp
-      next
-        show "vars_cls (add_mset (lit_of_glit K\<^sub>G) (cls_of_gcls D\<^sub>G) \<cdot> Var) \<inter>
-          vars_cls (add_mset (lit_of_glit L\<^sub>G) (cls_of_gcls C\<^sub>G) \<cdot> Var) = {}"
-          by simp
-      next
-        show "SCL_FOL.is_imgu Var {{atm_of (lit_of_glit K\<^sub>G) \<cdot>a Var, atm_of (lit_of_glit L\<^sub>G) \<cdot>a Var}}"
-          by (simp add: \<open>L\<^sub>G = - K\<^sub>G\<close> atm_of_lit_of_glit_conv SCL_FOL.is_imgu_def
-              SCL_FOL.is_unifiers_def SCL_FOL.is_unifier_def)
-      next
-        show "is_grounding_merge Var
-          (vars_cls (add_mset (lit_of_glit K\<^sub>G) (cls_of_gcls D\<^sub>G) \<cdot> Var))
-          (rename_subst_domain Var Var)
-          (vars_cls (add_mset (lit_of_glit L\<^sub>G) (cls_of_gcls C\<^sub>G) \<cdot> Var))
-          (rename_subst_domain Var Var)"
-          by (simp add: is_grounding_merge_def)
-      qed
-
-      thus "scl_fol.scl N \<beta> S S'"
-        unfolding scl_fol.scl_def by argo
-    next
-      fix S'' :: "('f, 'v) SCL_FOL.state"
-      assume "scl_fol.conflict N \<beta> S' S''"
-
-      moreover have "\<nexists>S''. scl_fol.conflict N \<beta> S' S''"
-        unfolding S'_def \<C>'_def \<open>\<C>\<^sub>G' = Some (C\<^sub>G + D\<^sub>G)\<close> by (simp add: scl_fol.conflict.simps)
-
-      ultimately show False
-        by metis
-    qed
-
-    ultimately show ?thesis
-      unfolding scl_fol.regular_scl_def by argo
-  next
-    case step_hyps: (backjump L\<^sub>G K\<^sub>G D\<^sub>G)
-
-    have "U' = finsert (add_mset (lit_of_glit K\<^sub>G) (cls_of_gcls D\<^sub>G)) U"
-      unfolding U_def U'_def \<open>U\<^sub>G' = finsert (add_mset K\<^sub>G D\<^sub>G) U\<^sub>G\<close>
-      by (simp add: cls_of_gcls_def)
-
-    have "\<C> = Some (add_mset (lit_of_glit K\<^sub>G) (cls_of_gcls D\<^sub>G), Var)"
-      unfolding \<C>_def \<open>\<C>\<^sub>G = Some (add_mset K\<^sub>G D\<^sub>G)\<close> option.map
-      by (simp add: cls_of_gcls_def)
-
-    have "\<C>' = None"
-      unfolding \<C>'_def \<open>\<C>\<^sub>G' = None\<close> option.map ..
-
-    have "\<not> Ex (scl_fol.conflict N \<beta> S)"
-      using \<open>\<C>\<^sub>G = Some (add_mset K\<^sub>G D\<^sub>G)\<close> nex_conflict_if_alread_in_conflict by metis
-
-    moreover have "scl_fol.reasonable_scl N \<beta> S S'"
-      unfolding scl_fol.reasonable_scl_def
-    proof (intro conjI impI notI ; (elim exE) ?)
-      have "scl_fol.backtrack N \<beta> S S'"
-        unfolding S_def S'_def \<open>U' = finsert (add_mset (lit_of_glit K\<^sub>G) (cls_of_gcls D\<^sub>G)) U\<close>
-        unfolding \<open>\<C> = Some (add_mset (lit_of_glit K\<^sub>G) (cls_of_gcls D\<^sub>G), Var)\<close>
-        unfolding \<open>\<C>' = None\<close>
-        sketch (rule scl_fol.backtrackI)
-      proof (rule scl_fol.backtrackI)
-        show "\<Gamma> = trail_decide ([] @ \<Gamma>') (lit_of_glit L\<^sub>G)"
-          unfolding \<Gamma>_def \<Gamma>'_def \<open>\<Gamma>\<^sub>G = (L\<^sub>G, None) # \<Gamma>\<^sub>G'\<close> decide_lit_def
-          by simp
-      next
-        show "lit_of_glit L\<^sub>G = - (lit_of_glit K\<^sub>G \<cdot>l Var)"
-          unfolding \<open>L\<^sub>G = - K\<^sub>G\<close>
-          by (cases K\<^sub>G) (simp_all add: lit_of_glit_def)
-      next
-        have "trail_consistent \<Gamma>\<^sub>G"
-          using \<open>trail_consistent (fst S\<^sub>G)\<close>[unfolded S\<^sub>G_def prod.sel] .
-        hence "\<not> trail_defined_lit \<Gamma>\<^sub>G' L\<^sub>G"
-          unfolding \<open>\<Gamma>\<^sub>G = (L\<^sub>G, None) # \<Gamma>\<^sub>G'\<close>
-          by (auto elim: trail_consistent.cases)
-        hence "\<not> trail_defined_lit \<Gamma>\<^sub>G' K\<^sub>G"
-          unfolding \<open>L\<^sub>G = - K\<^sub>G\<close>
-          by (simp add: trail_defined_lit_def) 
-        hence "\<not> trail_false_lit \<Gamma>\<^sub>G' K\<^sub>G"
-          using trail_defined_lit_iff_true_or_false by metis
-        hence "\<not> trail_false_cls \<Gamma>\<^sub>G' (add_mset K\<^sub>G D\<^sub>G)"
-          by (simp add: trail_false_cls_def)
-        hence "\<not> trail_false_cls \<Gamma>' (add_mset (lit_of_glit K\<^sub>G) (cls_of_gcls D\<^sub>G))"
-          by (metis (no_types, lifting) \<Gamma>'_def cls_of_gcls_def image_mset_add_mset
-              trail_false_cls_nonground_iff_trail_false_cls_ground)
-        thus "\<nexists>\<gamma>. is_ground_cls (add_mset (lit_of_glit K\<^sub>G) (cls_of_gcls D\<^sub>G) \<cdot> \<gamma>) \<and>
-          trail_false_cls \<Gamma>' (add_mset (lit_of_glit K\<^sub>G) (cls_of_gcls D\<^sub>G) \<cdot> \<gamma>)"
-          by simp
-      qed
-
-      thus "scl_fol.scl N \<beta> S S'"
-        unfolding scl_fol.scl_def by argo
-    next
-      fix S'' :: "('f, 'v) SCL_FOL.state"
-      assume "scl_fol.decide N \<beta> S S'"
-      thus False
-        unfolding S_def \<open>\<C> = Some (add_mset (lit_of_glit K\<^sub>G) (cls_of_gcls D\<^sub>G), Var)\<close>
-        by (auto elim!: scl_fol.decide.cases)
-    qed
-
-    ultimately show ?thesis
-      unfolding scl_fol.regular_scl_def by argo
+    show "ord_res_11 N S S'"
+      using step .
   qed
-qed
-
-
-section \<open>SCL(FOL)-0\<close>
-
-lemma "grounding_of_clss (fset (cls_of_gcls |`| N)) = fset (cls_of_gcls |`| N)"
-proof (rule scl_fol.grounding_of_clss_ground)
-  show "is_ground_clss (fset (cls_of_gcls |`| N::('a, 'b) Term.term literal multiset fset))"
-    by (simp add: is_ground_clss_def)
-qed
-
-thm scl_fol.correct_termination_regular_scl_run[of "cls_of_gcls |`| N" "term_of_gterm \<beta>" for N \<beta>]
-
-inductive scl_fol_0_step where
-  "\<nexists>\<gamma>. state_conflict S = Some ({#}, \<gamma>) \<Longrightarrow>
-    \<exists>C |\<in>| N. \<not> trail_true_cls (state_trail S) (cls_of_gcls C) \<Longrightarrow>
-    scl_fol.regular_scl (cls_of_gcls |`| N) (term_of_gterm \<beta>) S S' \<Longrightarrow>
-    scl_fol_0_step (N, \<beta>, S) (N, \<beta>, S')"
-
-fun scl_fol_0_final :: "'f gterm clause fset \<times> 'f gterm \<times> ('f, 'v) SCL_FOL.state \<Rightarrow> bool" where
-  "scl_fol_0_final (N, \<beta>, \<Gamma>, U, \<C>) \<longleftrightarrow>
-    (\<exists>\<gamma>. \<C> = Some ({#}, \<gamma>)) \<or> (\<forall>C |\<in>| N. trail_true_cls \<Gamma> (cls_of_gcls C))"
-
-interpretation scl_fol_semantics: semantics where
-  step = scl_fol_0_step and
-  final = scl_fol_0_final
-proof unfold_locales
-  fix S :: "'f gterm clause fset \<times> 'f gterm \<times> ('f, 'v) SCL_FOL.state"
-  obtain N \<beta> \<Gamma> U \<C> where
-    S_def: "S = (N, \<beta>, \<Gamma>, U, \<C>)"
-    by (metis prod.exhaust)
-
-  assume "scl_fol_0_final S"
-  hence "(\<exists>\<gamma>. \<C> = Some ({#}, \<gamma>)) \<or> (\<forall>C |\<in>| N. trail_true_cls \<Gamma> (cls_of_gcls C))"
-    unfolding S_def by simp
-  hence "\<nexists>S'. scl_fol_0_step S S'"
-  proof (elim disjE exE conjE)
-    fix \<gamma>
-    assume "\<C> = Some ({#}, \<gamma>)"
-    thus ?thesis
-      by (auto simp: S_def elim: scl_fol_0_step.cases)
-  next
-    assume "\<forall>C|\<in>|N. trail_true_cls \<Gamma> (cls_of_gcls C)"
-    then show ?thesis
-      by (auto simp: S_def elim: scl_fol_0_step.cases)
-  qed
-  thus "finished scl_fol_0_step S"
-    by (simp add: finished_def)
+next
+  show "state_of_gstate ({||}, {||}, [], None) = SCL_FOL.initial_state"
+    by simp
 qed
 
 end
